set up environment to start proofs

ironfleet/src/Dafny/Distributed/Protocol/ZooKeeper/PerformamceProof/ProofEmptyDiff.dfy
@@ -30,16 +30,33 @@ import opened ZooKeeper_TimestampedDistributedSystem
 import opened Zookeeper_PerformancePredicates
 
 
-
-lemma ZK_Performance_Guarantee(config:Config, tlb:seq<TLS_State>, f:int)
+/* Main theorem */
+lemma theorem_ZK_Performance_Guarantee(config:Config, tlb:seq<TLS_State>, f:int)
     requires SeqIsUnique(config);
     requires ValidTLSBehavior(config, tlb, f)
     requires Performance_Assumption_EmptyDiff(tlb)
-    ensures Performance_Guarantee_EmptyDiff(tlb);
+    ensures Performance_Guarantee_EmptyDiff(tlb)
 {
     // TODO
     assume false;
 }
 
 
+predicate FollowerInfo_Message_Guarantee(tls:TLS_State)
+{
+    var perf_formula := SendFI;
+    forall ep | ep in tls.t_environment.channels :: (
+        forall pkt | pkt in tls.t_environment.channels[ep].channel
+        :: pkt.msg.ts == perf_formula
+    )
+}
+
+lemma lemma_FollowerInfo_Message_Guarantee(config:Config, tlb:seq<TLS_State>, f:int)
+    requires SeqIsUnique(config);
+    requires ValidTLSBehavior(config, tlb, f)
+    requires Performance_Assumption_EmptyDiff(tlb)
+    ensures forall i | 0 <= i < |tlb| :: FollowerInfo_Message_Guarantee(tlb[i])
+{
+    assume false;
+}
 }
